Finish theories with typeclass and some changes

typeclass/Interfaces/assetmapping_spl_int.v
@@ -6,9 +6,10 @@ Require Export Coq.Lists.List.
 Class AssetMapping (A N m: Type): Type :=
 {
   (*====================functions=======================*)
-  assetRef  : set A -> set A -> Prop;
-  wfProduct : set A -> Prop;
-  aMR       : m -> m -> Prop;
+  assetRef    : set A -> set A -> Prop;
+  wfProduct   : set A -> Prop;
+  aMR         : m -> m -> Prop;
+  my_set_union: set A -> set A -> set A;
 
   (*===========Axioms - Lemmas - Theorems====================*)
   assetRefinementReflexivity : 
@@ -16,14 +17,12 @@ Class AssetMapping (A N m: Type): Type :=
   assetRefinementTranstivity : 
     forall x y z: set A, 
       assetRef x y -> assetRef y z ->  assetRef x z;
-  as_dec                     : 
-      forall x y:A, {x = y} + {x <> y};
   asRefCompositional         :  
     forall (S1 : set A) (S2 : set A) (aSet : set A),
-      (assetRef S1 S2) /\ wfProduct (set_union as_dec S1 aSet) 
-        -> (wfProduct (set_union as_dec S2 aSet)) 
-          /\ assetRef (set_union as_dec S1 aSet) 
-             (set_union as_dec S2 aSet);
+      (assetRef S1 S2) /\ wfProduct (my_set_union S1 aSet) 
+        -> (wfProduct (my_set_union S2 aSet)) 
+          /\ assetRef (my_set_union S1 aSet) 
+             (my_set_union S2 aSet);
   assetMappingRefinement: 
     forall x y z: m, 
       aMR x x /\ aMR x y -> aMR y z ->  aMR x z;
