typeclass/Interfaces/assettheory_int.v
@@ -6,12 +6,16 @@ Require Export maps_int.
 
 Class AssetTheory (A N m: Type) {Mp: Maps A N m} : Type :=  
 {
+  (*====================functions=======================*)
+
   wfProduct: set N -> Prop;
+  assetRef : set N -> set N -> Prop;
+
+  (*===========Axioms - Lemmas - Theorems====================*)  
   ANdec_eq : 
     forall x y: A, {x = y} + {x <> y};
   Asset_dec : 
     forall x y: N, {x = y} + {x <> y};
-  assetRef: set N -> set N -> Prop;
   assetRefinement:
     forall x y z: set N, assetRef x x /\ 
       assetRef x y -> assetRef y z ->  assetRef x z;
@@ -21,10 +25,4 @@ Class AssetTheory (A N m: Type) {Mp: Maps A N m} : Type :=
         -> (wfProduct (union_t S2 aSet)) 
           /\ assetRef (union_t S1 aSet) 
              (union_t S2 aSet);
-  assetTest:
-  forall (S1 S2 x y : set N) (a b : N),
-    wfProduct x /\ (assetRef S1 S2) /\ (set_In a x) /\ 
-      (assetRef (set_add Asset_dec a nil) (set_add Asset_dec b nil))
-        /\ (x = set_add Asset_dec a S1) /\ (y = set_add Asset_dec b S2) 
-          -> assetRef x y 
 }. 
