typeclass/Interfaces/featuremodelsemantics_int.v
@@ -7,6 +7,8 @@ Require Export formulatheory_int.
 
 Class FeatureModelSemantics (FL F N: Type) {FormT: FormulaTheory FL N F} : Type :=
 {
+  (*====================functions=======================*)
+
   wfFM        : F -> Prop;
   satImpConsts: F -> set N -> Prop;
   satExpConsts: F -> set N -> Prop;
@@ -14,10 +16,15 @@ Class FeatureModelSemantics (FL F N: Type) {FormT: FormulaTheory FL N F} : Type 
   refines     : F -> F -> Prop;
   refines2    : F -> F -> Prop;
   ns          : F -> set N;
-  wtFormRefinement : forall (abs : F) (con : F), forall (name : N),
-    set_In name (ns abs) -> set_In name (ns con) /\ (wfTree abs) /\
-      (wfTree con) -> (forall (f : FL), (wt (ns abs) f) -> (wt (ns con) f));
-  notMember : forall (fm : F), wfFM fm = True -> ( forall (opt : N), 
-   ~(set_In opt ( ns fm)) -> (forall (conf : set N), 
-    set_In conf (semantics fm) -> ~ (set_In opt (conf))))
+
+  (*===========Axioms - Lemmas - Theorems====================*)  
+
+  wtFormRefinement :
+    forall (abs : F) (con : F), forall (name : N),
+      set_In name (ns abs) -> set_In name (ns con) /\ (wfTree abs) /\
+        (wfTree con) -> (forall (f : FL), (wt (ns abs) f) -> (wt (ns con) f));
+  notMember : 
+    forall (fm : F), wfFM fm = True -> ( forall (opt : N), 
+      ~(set_In opt ( ns fm)) -> (forall (conf : set N), 
+        set_In conf (semantics fm) -> ~ (set_In opt (conf))))
 }.  
