typeclass/Interfaces/formulatheory_int.v
@@ -5,26 +5,39 @@ Require Export Coq.Classes.RelationClasses.
 
 Class FormulaTheory (FL N F: Type) : Type :=
 {
-  names: FL -> set N;
-  wfTree: F -> Prop;
-  names_: F -> set N;
-  wt: set N -> FL -> Prop;
-  wtFormulae: F -> Prop;
-  satisfies: FL -> set N -> Prop;
-  name_dec : forall x y:N, {x = y} + {x <> y};
-  formNames: forall (fm : F) (f : FL),  
-    (wt (names_ fm) f) -> ( forall (n : N),
-      set_In n (names f) -> set_In n (names_ fm));
-  formNames2 : forall (fm : F) (f : FL) (n: N),
-    (wt (names_ fm) f) /\ (~(set_In n (names_ fm))) 
-      -> (~(set_In n (names f)));
-  satisfies1 : forall (f: FL) (c : set N) (n : N),
-    ~(set_In n (names f)) -> satisfies f c =
-      satisfies f (set_add name_dec n c);
-  satisfies2 : forall (f: FL) (c : set N) (n : N),
-    ~(set_In n (names f)) -> satisfies f c = 
-      satisfies f (set_remove name_dec n c);
-  wtFormSameFeature : forall (abs : F) (con : F), (names_ abs = names_ con
-  /\ (wfTree abs) /\ (wfTree con) -> forall (f : FL), (wt (names_ abs) f)
-  ->  (wt (names_ con) f))
+  (*====================functions=======================*)
+
+  names        : FL -> set N;
+  wfTree       : F -> Prop;
+  names_       : F -> set N;
+  wt           : set N -> FL -> Prop;
+  wtFormulae   : F -> Prop;
+  satisfies    : FL -> set N -> Prop;
+  my_set_add   : N -> set N -> set N;
+  my_set_remove: N -> set N -> set N;
+
+  (*===========Axioms - Lemmas - Theorems====================*)  
+
+  name_dec : 
+    forall x y:N, {x = y} + {x <> y};
+  formNames: 
+    forall (fm : F) (f : FL),  
+      (wt (names_ fm) f) -> ( forall (n : N),
+        set_In n (names f) -> set_In n (names_ fm));
+  formNames2 : 
+    forall (fm : F) (f : FL) (n: N),
+      (wt (names_ fm) f) /\ (~(set_In n (names_ fm))) 
+        -> (~(set_In n (names f)));
+  satisfies1 : 
+    forall (f: FL) (c : set N) (n : N),
+      ~(set_In n (names f)) -> satisfies f c =
+        satisfies f (my_set_add n c);
+  satisfies2 : 
+    forall (f: FL) (c : set N) (n : N),
+      ~(set_In n (names f)) -> satisfies f c = 
+        satisfies f (my_set_remove n c);
+  wtFormSameFeature :
+    forall (abs : F) (con : F), (names_ abs = names_ con
+      /\ (wfTree abs) /\ (wfTree con) -> forall (f : FL), (wt (names_ abs) f)
+        ->  (wt (names_ con) f))
 }.
