typeclass/Instances/featuremodelsemantics_inst.v
@@ -11,7 +11,7 @@ Require Export formulatheory_proofs.
 Import FormulaTheory.
 Import FeatureModelSemantics.
 
-Instance FeatureModelSemantics_Int : FeatureModelSemantics Formula FM Name:= 
+Program Instance FeatureModelSemantics_Int : FeatureModelSemantics Formula FM Name:= 
 {
   wfFM:= wfFM_func;
   satImpConsts:= satImpConsts_func;
@@ -21,11 +21,24 @@ Instance FeatureModelSemantics_Int : FeatureModelSemantics Formula FM Name:=
   refines2:= refines_func;
   ns := nsf_func
 
-}. Proof.
+}. Next Obligation.
 { (*wtFormRefinement*)
-  admit.
+  induction f.
+  + simpl; tauto.
+  + simpl; tauto.
+  + simpl. rewrite name in H0.
+    rewrite n. apply H0. 
+  + simpl; tauto.
+  + simpl in H1. destruct H1. split.
+    - apply IHf1. apply H1.
+    - apply IHf2. apply H4.
+  + simpl in H1.  split. 
+    - apply IHf1. destruct H1. apply H1.
+    - apply IHf2. destruct H1. apply H4.
 
-} { (*notMember*)
+} Qed.
+  Next Obligation.
+{ (*notMember*)
     intros.
     unfold not in H.
     unfold not. 
@@ -40,4 +53,4 @@ Instance FeatureModelSemantics_Int : FeatureModelSemantics Formula FM Name:=
     + destruct fm. destruct f.
       - simpl in H1. apply H1.
       - simpl in H. apply H0. left. rewrite n0. reflexivity.
-} Admitted.
+} Qed.
