typeclass/Instances/formulatheory_inst.v
@@ -1,14 +1,15 @@
-Require Export Coq.Lists.ListSet.
+Require Export Coq.Lists.ListSet. 
+Require Export Coq.Classes.SetoidDec.
 Require Export Coq.Lists.List.
 Require Export Coq.Bool.Bool.
-Require Export Coq.Classes.RelationClasses.
+Require Export Coq.Classes.RelationClasses. 
 Require Export formulatheory_def.
 Require Export formulatheory_proofs.
 Require Export formulatheory_int.
 Import FormulaTheory.
 
 
-Instance FormulaTheory_Ins: FormulaTheory Formula Name FM := 
+Program Instance FormulaTheory_Ins: FormulaTheory Formula Name FM := 
   {
   names:= names_func;
   wfTree:= wfTree_func;
@@ -16,80 +17,105 @@ Instance FormulaTheory_Ins: FormulaTheory Formula Name FM :=
   wt:= wt_func;
   wtFormulae:= wtFormulae_func;
   satisfies:= satisfies_func;
+  my_set_add := my_set_add_func;
+  my_set_remove := my_set_remove_func;
 
-}. Proof.
+}.  Next Obligation.
 { (*name_dec*)
   apply name_dec_axiom.
 
-} { (*formNames*)
+} Qed. 
+  Next Obligation.
+{ (*formNames*)
   induction f.
-    + simpl; tauto.
-    + simpl; tauto.
-    + simpl. intros. intuition. rewrite H1 in H. apply H.
-    + simpl. tauto.
-    + simpl. intros H ; destruct H. intros. apply set_union_elim in H1. inversion H1.
-      - apply IHf1. apply H. apply H2.
-      - apply set_diff_elim1 in H2. apply IHf2. apply H0. apply H2.
-    + simpl. intros H. destruct H. intros. apply set_union_elim in H1. inversion H1.
+    + simpl in H0. contradiction.
+    + simpl in H0. contradiction.
+    + simpl in H, H0. intuition. rewrite H1 in H. apply H.
+    + simpl in H, H0. intuition.
+    + simpl in H. destruct H. intuition. simpl in H0.
+    apply set_union_elim in H0. inversion H0.
+      - apply H2. apply H4. 
+      - apply set_diff_elim1 in H4. apply H3. apply H4.
+    + simpl in H. destruct H. simpl in H0. apply set_union_elim in H0.
+      inversion H0.
       - apply IHf1. apply H. apply H2. 
-      - apply set_diff_elim1 in H2. apply IHf2. apply H0. apply H2.
+      - apply set_diff_elim1 in H2. apply IHf2. 
+        * apply H1.
+        * apply H2.
 
-} { (*formNames2*)
+} Qed. 
+  Next Obligation.
+{ (*formNames2*)
   unfold not.
   induction f.
     + simpl; tauto.
     + simpl; tauto.
-    + simpl. intros. intuition. rewrite H in H1. apply H2. apply H1.
+    + simpl in H. unfold not in H0. intros.
+      simpl in H1. intuition. apply H0. rewrite <- H2. apply H.
     + simpl; tauto.
-    + simpl. intros. destruct H; destruct H. apply set_union_elim in H0. inversion H0.
-      - apply (IHf1 n). intuition. apply H3.
-      - apply set_diff_elim1 in H3. apply (IHf2 n). intuition. apply H3. 
-    + simpl. intros. destruct H. destruct H. apply set_union_elim in H0. inversion H0.
-      - apply (IHf1 n). intuition. apply H3.
-      - apply set_diff_elim1 in H3. apply (IHf2 n). intuition. apply H3.
+    + simpl. intros. simpl in H. destruct H. apply set_union_elim in H1.
+      inversion H1.
+      - apply IHf1.
+        * apply H.
+        * apply H3.
+      - apply set_diff_elim1 in H3. apply IHf2. 
+        * apply H2.
+        * apply H3.
+   + simpl. intros. simpl in H. destruct H. apply set_union_elim in H1.
+      inversion H1.
+      - apply IHf1.
+        * apply H.
+        * apply H3.
+      - apply set_diff_elim1 in H3. apply IHf2. 
+        * apply H2.
+        * apply H3.
 
-} { (*satisfies1*)
+} Qed. 
+  Next Obligation.  { (*satisfies1*) 
     induction f. 
-  + simpl; intros; reflexivity.
-  + simpl; intros; reflexivity.
-  + simpl. intros. intuition. apply H1 in H0. 
+  + simpl; reflexivity.
+  + simpl; reflexivity.
+  + simpl. simpl in H. unfold not in H. intuition. apply H1 in H0. 
     - contradiction. 
     - rewrite n. rewrite n0. reflexivity.
-  + simpl. intros. apply not_compat. apply (IHf c). apply H.
+  + simpl. intros. apply not_compat. apply IHf. apply H.
   + simpl. intros. apply set_union_elim_not in H. destruct H as [H1 H2]. 
-    specialize (IHf1 c n). specialize (IHf2 c n).
+    specialize IHf1. specialize IHf2.
     apply set_diff_elim_not in H2. inversion H2.
     -  apply IHf1 in H1. apply IHf2 in H. rewrite H1.
       rewrite H. reflexivity.
     - contradiction.
  + simpl. intros. apply set_union_elim_not in H. destruct H as [H1 H2]. 
-    specialize (IHf1 c n). specialize (IHf2 c n).
+    specialize IHf1. specialize IHf2.
     apply set_diff_elim_not in H2. inversion H2.
     -  apply IHf1 in H1. apply IHf2 in H. rewrite H1.
       rewrite H. reflexivity.
-    - contradiction.
-
-} { (*satisfies2*)
-  induction f.
-  + simpl. intros. reflexivity.
-  + simpl. intros. reflexivity.
-  + simpl. intros. intuition. apply H1 in H0. 
+    - contradiction. 
+} Qed.
+  Next Obligation. 
+{ (*satisfies2*)
+   induction f. 
+  + simpl; reflexivity.
+  + simpl; reflexivity.
+  + simpl. simpl in H. unfold not in H. intuition. apply H1 in H0. 
     - contradiction. 
     - rewrite n. rewrite n0. reflexivity.
-  + simpl. intros. apply not_compat. apply (IHf c). apply H. 
+  + simpl. intros. apply not_compat. apply IHf. apply H.
   + simpl. intros. apply set_union_elim_not in H. destruct H as [H1 H2]. 
-    specialize (IHf1 c n). specialize (IHf2 c n).
+    specialize IHf1. specialize IHf2.
     apply set_diff_elim_not in H2. inversion H2.
     -  apply IHf1 in H1. apply IHf2 in H. rewrite H1.
       rewrite H. reflexivity.
     - contradiction.
  + simpl. intros. apply set_union_elim_not in H. destruct H as [H1 H2]. 
-    specialize (IHf1 c n). specialize (IHf2 c n).
+    specialize IHf1. specialize IHf2.
     apply set_diff_elim_not in H2. inversion H2.
     -  apply IHf1 in H1. apply IHf2 in H. rewrite H1.
       rewrite H. reflexivity.
-    - contradiction.
-} { (*wtFormSameFeature*)
+    - contradiction. 
+} Qed.
+  (*Next Obligation.
+{ (*wtFormSameFeature*)
   intros.
   destruct H as [equals_abs_con wf_abs_con].
   destruct wf_abs_con as [wf_abs wf_con].
@@ -101,4 +127,4 @@ Instance FormulaTheory_Ins: FormulaTheory Formula Name FM :=
     + rewrite equals_abs_con in H0. apply H0. 
     + rewrite equals_abs_con in H0. apply H0. 
 
-} Qed.
+} Qed. *)
